src/ocaml-output/FStar_Syntax_Embeddings.ml
@@ -13,6 +13,7 @@ type norm_step =
   | UnfoldFully of Prims.string Prims.list 
   | UnfoldAttr of Prims.string Prims.list 
   | UnfoldQual of Prims.string Prims.list 
+  | UnfoldNamespace of Prims.string Prims.list 
   | NBE 
   | Unmeta 
 let (uu___is_Simpl : norm_step -> Prims.bool) =
@@ -53,6 +54,12 @@ let (uu___is_UnfoldQual : norm_step -> Prims.bool) =
     match projectee with | UnfoldQual _0 -> true | uu___ -> false
 let (__proj__UnfoldQual__item___0 : norm_step -> Prims.string Prims.list) =
   fun projectee -> match projectee with | UnfoldQual _0 -> _0
+let (uu___is_UnfoldNamespace : norm_step -> Prims.bool) =
+  fun projectee ->
+    match projectee with | UnfoldNamespace _0 -> true | uu___ -> false
+let (__proj__UnfoldNamespace__item___0 :
+  norm_step -> Prims.string Prims.list) =
+  fun projectee -> match projectee with | UnfoldNamespace _0 -> _0
 let (uu___is_NBE : norm_step -> Prims.bool) =
   fun projectee -> match projectee with | NBE -> true | uu___ -> false
 let (uu___is_Unmeta : norm_step -> Prims.bool) =
@@ -1379,6 +1386,8 @@ let (steps_UnfoldAttr : FStar_Syntax_Syntax.term) =
   FStar_Syntax_Syntax.tconst FStar_Parser_Const.steps_unfoldattr
 let (steps_UnfoldQual : FStar_Syntax_Syntax.term) =
   FStar_Syntax_Syntax.tconst FStar_Parser_Const.steps_unfoldqual
+let (steps_UnfoldNamespace : FStar_Syntax_Syntax.term) =
+  FStar_Syntax_Syntax.tconst FStar_Parser_Const.steps_unfoldnamespace
 let (steps_NBE : FStar_Syntax_Syntax.term) =
   FStar_Syntax_Syntax.tconst FStar_Parser_Const.steps_nbe
 let (steps_Unmeta : FStar_Syntax_Syntax.term) =
@@ -1449,7 +1458,17 @@ let (e_norm_step : norm_step embedding) =
                    uu___4 rng FStar_Pervasives_Native.None norm in
                  FStar_Syntax_Syntax.as_arg uu___3 in
                [uu___2] in
-             FStar_Syntax_Syntax.mk_Tm_app steps_UnfoldQual uu___1 rng) in
+             FStar_Syntax_Syntax.mk_Tm_app steps_UnfoldQual uu___1 rng
+         | UnfoldNamespace l ->
+             let uu___1 =
+               let uu___2 =
+                 let uu___3 =
+                   let uu___4 =
+                     let uu___5 = e_list e_string in embed uu___5 l in
+                   uu___4 rng FStar_Pervasives_Native.None norm in
+                 FStar_Syntax_Syntax.as_arg uu___3 in
+               [uu___2] in
+             FStar_Syntax_Syntax.mk_Tm_app steps_UnfoldNamespace uu___1 rng) in
   let un t0 w norm =
     let t = unmeta_div_results t0 in
     lazy_unembed printer1 emb_t_norm_step t t_norm_step
@@ -1559,6 +1578,19 @@ let (e_norm_step : norm_step embedding) =
                        FStar_Compiler_Effect.op_Less_Bar
                          (fun uu___4 -> FStar_Pervasives_Native.Some uu___4)
                          (UnfoldQual ss))
+              | (FStar_Syntax_Syntax.Tm_fvar fv, (l, uu___2)::[]) when
+                  FStar_Syntax_Syntax.fv_eq_lid fv
+                    FStar_Parser_Const.steps_unfoldnamespace
+                  ->
+                  let uu___3 =
+                    let uu___4 =
+                      let uu___5 = e_list e_string in unembed uu___5 l in
+                    uu___4 w norm in
+                  FStar_Compiler_Util.bind_opt uu___3
+                    (fun ss ->
+                       FStar_Compiler_Effect.op_Less_Bar
+                         (fun uu___4 -> FStar_Pervasives_Native.Some uu___4)
+                         (UnfoldNamespace ss))
               | uu___2 ->
                   (if w
                    then
