ulib/tactics_ml/FStar_Tactics_Builtins.ml
@@ -39,6 +39,7 @@ let tr1 = function
           | UnfoldFully ss -> EMB.UnfoldFully ss
           | UnfoldAttr  ss -> EMB.UnfoldAttr  ss
           | UnfoldQual  ss -> EMB.UnfoldQual  ss
+          | UnfoldNamespace  ss -> EMB.UnfoldNamespace  ss
 let rt1 = function
           | EMB.Simpl          -> Simpl
           | EMB.Weak           -> Weak
@@ -55,6 +56,7 @@ let rt1 = function
           | EMB.UnfoldFully ss -> UnfoldFully ss
           | EMB.UnfoldAttr  ss -> UnfoldAttr  ss
           | EMB.UnfoldQual  ss -> UnfoldQual  ss
+          | EMB.UnfoldNamespace  ss -> UnfoldNamespace  ss
 
 (* the one plugins actually use *)
 let e_norm_step' : norm_step EMB.embedding =
