src/syntax/FStar.Syntax.Embeddings.fsti
@@ -42,6 +42,7 @@ type norm_step =
     | UnfoldFully of list string
     | UnfoldAttr  of list string
     | UnfoldQual  of list string
+    | UnfoldNamespace of list string    
     | NBE
     | Unmeta
 
