ulib/FStar.Pervasives.fst
@@ -57,6 +57,7 @@ type norm_step =
   | UnfoldFully : list string -> norm_step
   | UnfoldAttr : list string -> norm_step // Unfold definitions marked with the given attributes
   | UnfoldQual : list string -> norm_step
+  | UnfoldNamespace : list string -> norm_step
   | Unmeta : norm_step
 
 irreducible
@@ -100,6 +101,9 @@ let delta_attr s = UnfoldAttr s
 
 irreducible
 let delta_qualifier s = UnfoldAttr s
+
+irreducible
+let delta_namespace s = UnfoldNamespace s
 
 irreducible
 let unmeta = Unmeta
